first pass at juicy_machine

concurrency/juicy/juicy_machine.v
@@ -12,7 +12,7 @@ Require Import VST.concurrency.common.scheduler.
 Require Import VST.concurrency.common.HybridMachineSig.
 Require Import VST.concurrency.common.addressFiniteMap. (*The finite maps*)
 Require Import VST.concurrency.common.threads_lemmas.
-(*Require Import VST.concurrency.juicy.rmap_locking.*)
+Require Import VST.concurrency.juicy.rmap_locking.
 Require Import VST.concurrency.common.lksize.
 Require Import VST.concurrency.common.semantics.
 Require Import VST.concurrency.common.permjoin.
@@ -104,23 +104,27 @@ Module Concur.
     Notation thread_pool := (@ThreadPool.t _ _ OrdinalThreadPool).
 
     (** Machine Variables*)
-    Definition lp_id : tid:= (0)%nat. (*lock pool thread id*)
+    Definition lp_id : tid := (0)%nat. (*lock pool thread id*)
 
     (** Invariants*)
     (** The state respects the memory*)
-(*    Definition access_cohere' m phi:= forall loc,
-        Mem.perm_order'' (max_access_at m loc) (perm_of_res (phi @ loc)).*)
+    Definition contents_cohere m phi := forall loc, contents_cohere m loc (phi @ loc).
+    Definition access_cohere m phi := forall loc, access_cohere m loc (phi @ loc).
+    Definition access_cohere' m phi := forall loc,
+        Mem.perm_order'' (max_access_at m loc) (perm_of_res (phi @ loc)).
+    Definition max_access_cohere m phi := forall loc, max_access_cohere m loc (phi @ loc).
+    Definition alloc_cohere m (phi : juicy_mem.rmap) := forall loc, (loc.1 >= Mem.nextblock m)%positive → phi !! loc = None.
 
     (* This is similar to the coherence of juicy memories, *
      * but for entire machines. It is slighly weaker in one way:
      * - acc_coh is looser and only talks about maxcoh.
      * - else acc_coh might be redundant with max_coh IDK... x*)
     Record mem_cohere' m phi :=
-      { cont_coh: forall loc, contents_cohere m loc (resource_at phi loc);
+      { cont_coh: contents_cohere m phi;
         (*acc_coh: access_cohere m phi;*)
         (*acc_coh: access_cohere' m phi;*)
-        max_coh: forall loc, max_access_cohere m loc (resource_at phi loc);
-        all_coh: forall loc, (loc.1 >= Mem.nextblock m)%positive → phi !! loc = None
+        max_coh: max_access_cohere m phi;
+        all_coh: alloc_cohere m phi
       }.
     Definition mem_thcohere (tp : thread_pool) m :=
       forall tid (cnt: containsThread tp tid), mem_cohere' m (getThreadR cnt).
@@ -234,6 +238,7 @@ Qed.
         join_locks tp r1 ->
         (Some r0 : optionUR (resource_map.rmapUR _ _)) ⋅ r1 ≡ Some r2 ->
         r2 ⋅ (extraRes tp) ≡ r ->
+        ✓ r ->
         join_all tp r.
 
     (* Should we do this at the logic level? *)
@@ -289,6 +294,11 @@ Qed.
       }.
 
     Definition mem_compatible_with := mem_compatible_with'.
+
+    Lemma mem_compatible_with_valid : forall tp m phi, mem_compatible_with tp m phi -> ✓ phi.
+    Proof.
+      by intros ??? [[]].
+    Qed.
 
     Definition mem_compatible tp m := ex (mem_compatible_with tp m).
 
@@ -380,7 +390,7 @@ Qed.
     Proof. intros. eapply mem_compatible_locks_ltwritable; auto. Qed.
 
 
-    Lemma compatible_lockRes_join:
+(*    Lemma compatible_lockRes_join:
       forall (js : thread_pool) (m : mem),
         mem_compatible js m ->
         forall (l1 l2 : address) (phi1 phi2 : rmap),
@@ -393,7 +403,7 @@ Qed.
            inversion Hcompat.
            inversion juice_join0; subst.
            unfold join_locks in H2.
-           clear - Hneq H2 H H0. unfold lockRes,lockGuts in H, H0.
+           clear - Hneq H2 H H0.
            apply AMap.find_2 in H. apply AMap.find_2 in H0.
   assert (forall x e, AMap.MapsTo x e (lset js) <->
                SetoidList.InA (@AMap.eq_key_elt lock_info) (x,e) (AMap.elements (lset js))). {
@@ -404,9 +414,10 @@ Qed.
   assert (SetoidList.InA (@AMap.eq_key_elt lock_info) (l2, Some phi2) el).
    apply H1; auto.
  clear - H2 H3 H4 Hneq.
+ 
  revert r1 H2 H3 H4; induction el; simpl; intros.
  inv H3.
- destruct H2 as [r2 [? ?]]. destruct a.
+ destruct a.
   assert (H8: joins (Some phi1) (Some phi2));
     [ | destruct H8 as [x H8]; destruct x; inv H8; eauto].
  inv H3; [ | inv H4].
@@ -461,7 +472,7 @@ Qed.
     Definition disjoint_lock_thread tp :=
       forall i loc r (cnti : containsThread tp i),
         lockRes tp loc = SSome r ->
-        joins (getThreadR cnti)r.
+        joins (getThreadR cnti)r.*)
 
     Variant invariant' (tp:t) := True. (* The invariant has been absorbed my mem_compat*)
      (* { no_race : disjoint_threads tp
@@ -476,8 +487,10 @@ Qed.
     (* What follows is the lemmas needed to construct a "personal" memory
        That is a memory with the juice and Cur of a particular thread. *)
 
+    Local Open Scope maps.
+
     Definition mapmap {A B} (def:B) (f:positive -> A -> B) (m:PMap.t A): PMap.t B:=
-      (def, PTree.map f m#2).
+      (def, PTree.map f m.2).
     (* You need the memory, to make a finite tree. *)
     Definition juice2Perm (phi:rmap)(m:mem): access_map:=
       mapmap (fun _ => None) (fun block _ => fun ofs => perm_of_res (phi @ (block, ofs)) ) (getMaxPerm m).
@@ -489,11 +502,11 @@ Qed.
           Proof. unfold isCanonical; reflexivity. Qed.
     Lemma juice2Perm_nogrow: forall phi m b ofs,
         Mem.perm_order'' (perm_of_res (phi @ (b, ofs)))
-                         ((juice2Perm phi m) !! b ofs).
+                         (PMap.get b (juice2Perm phi m) ofs).
     Proof.
       intros. unfold juice2Perm, mapmap, PMap.get.
       rewrite PTree.gmap.
-      destruct (((getMaxPerm m)#2) ! b) eqn: inBounds; simpl.
+      destruct (((getMaxPerm m).2) !! b) eqn: inBounds; simpl.
       - destruct ((perm_of_res (phi @ (b, ofs)))) eqn:AA; rewrite AA; simpl; try reflexivity.
         apply perm_refl.
       - unfold Mem.perm_order''.
@@ -501,11 +514,11 @@ Qed.
     Qed.
     Lemma juice2Perm_locks_nogrow: forall phi m b ofs,
         Mem.perm_order'' (perm_of_res_lock (phi @ (b, ofs)))
-                         ((juice2Perm_locks phi m) !! b ofs).
+                         (PMap.get b (juice2Perm_locks phi m) ofs).
     Proof.
       intros. unfold juice2Perm_locks, mapmap, PMap.get.
       rewrite PTree.gmap.
-      destruct (((getMaxPerm m)#2) ! b) eqn: inBounds; simpl.
+      destruct (((getMaxPerm m).2) !! b) eqn: inBounds; simpl.
       - destruct ((perm_of_res_lock (phi @ (b, ofs)))) eqn:AA; rewrite AA; simpl; try reflexivity.
         apply perm_refl.
       - unfold Mem.perm_order''.
@@ -536,17 +549,17 @@ Qed.
     Qed.
 
     Lemma Mem_canonical_useful: forall m loc k,
-        (Mem.mem_access m)#1 loc k = None.
+        (Mem.mem_access m).1 loc k = None.
     Proof. intros. destruct m; simpl in *.
            unfold PMap.get in nextblock_noaccess.
-           pose (b:= Pos.max (TreeMaxIndex (mem_access#2) + 1 )  nextblock).
-           assert (H1:  ~ Plt b nextblock).
-           { intros H. assert (HH:= Pos.le_max_r (TreeMaxIndex (mem_access#2) + 1) nextblock).
+           pose (b:= Pos.max (TreeMaxIndex (mem_access.2) + 1) nextblock).
+           assert (H1: ~ Plt b nextblock).
+           { intros H. assert (HH:= Pos.le_max_r (TreeMaxIndex (mem_access.2) + 1) nextblock).
              clear - H HH. unfold Pos.le in HH. unfold Plt in H.
              apply HH. eapply Pos.compare_gt_iff.
              auto. }
-           assert (H2 :( b > (TreeMaxIndex (mem_access#2)))%positive ).
-           { assert (HH:= Pos.le_max_l (TreeMaxIndex (mem_access#2) + 1) nextblock).
+           assert (H2 :( b > (TreeMaxIndex (mem_access.2)))%positive ).
+           { assert (HH:= Pos.le_max_l (TreeMaxIndex (mem_access.2) + 1) nextblock).
              apply Pos.lt_gt. eapply Pos.lt_le_trans; eauto.
              lia. }
            specialize (nextblock_noaccess b loc k H1).
@@ -554,50 +567,61 @@ Qed.
            assumption.
     Qed.
 
+    Lemma big_opL_In : forall {M : ofe} o {HM : Monoid o} A (f : A -> M) l a, In a l -> exists l', ([^o list] x ∈ l, f x) ≡ o (f a) l'.
+    Proof.
+      induction l; simpl; intros; first done.
+      destruct H as [-> | H]; eauto.
+      edestruct IHl as (l' & Heq); first done.
+      exists (o (f a) l').
+      rewrite monoid_proper; last apply Heq; last done.
+      rewrite !monoid_assoc.
+      apply monoid_proper; last done.
+      apply monoid_comm.
+    Qed.
+
+    Lemma join_list_not_none : forall {A : ora} (a : A) (l : list (option A)), In (Some a) l -> ([^op list] x ∈ l, x) <> None.
+    Proof.
+      intros.
+      eapply (big_opL_In id l) in H as (? & H).
+      rewrite /= Some_op_opM in H.
+      inversion H as [??? Heq|]; rewrite -Heq //.
+    Qed.
+
     Lemma juic2Perm_locks_correct:
       forall r m b ofs,
         max_access_cohere m r ->
-        perm_of_res_lock (r @ (b,ofs)) = (juice2Perm_locks r m) !! b ofs.
+        perm_of_res_lock (r @ (b,ofs)) = PMap.get b (juice2Perm_locks r m) ofs.
     Proof.
         intros.
         unfold juice2Perm_locks, mapmap.
         unfold PMap.get; simpl.
         rewrite PTree.gmap.
         rewrite PTree.gmap1; simpl.
-        destruct ((snd (Mem.mem_access m)) ! b) eqn:search; simpl.
+        destruct ((snd (Mem.mem_access m)) !! b) eqn:search; simpl.
         - auto.
         - generalize (H (b, ofs)) => /po_trans.
           move =>  /(_ (perm_of_res_lock (r @ (b, ofs)))) /(_ (perm_of_res_op2 _)).
           unfold max_access_at. unfold access_at. unfold PMap.get; simpl.
           rewrite search. rewrite Mem_canonical_useful.
-          unfold perm_of_res_lock. destruct ( r @ (b, ofs)); auto.
-          destruct k; auto. simpl.
-          destruct (perm_of_sh (Share.glb Share.Rsh sh)) eqn: HH; auto.
-          intros; exfalso; assumption.
+          destruct (perm_of_res_lock (r @ (b, ofs))); done.
     Qed.
 
     Lemma juic2Perm_correct:
       forall r m b ofs,
         access_cohere' m r ->
-        perm_of_res (r @ (b,ofs)) = (juice2Perm r m) !! b ofs.
+        perm_of_res (r @ (b,ofs)) = PMap.get b (juice2Perm r m) ofs.
     Proof.
         intros.
         unfold juice2Perm, mapmap.
         unfold PMap.get; simpl.
         rewrite PTree.gmap.
         rewrite PTree.gmap1; simpl.
-        destruct ((snd (Mem.mem_access m)) ! b) eqn:search; simpl.
+        destruct ((snd (Mem.mem_access m)) !! b) eqn:search; simpl.
         - auto.
         - generalize (H (b, ofs)).
           unfold max_access_at. unfold access_at. unfold PMap.get; simpl.
           rewrite search. rewrite Mem_canonical_useful.
-          unfold perm_of_res. destruct ( r @ (b, ofs)).
-          destruct (eq_dec sh Share.bot); auto; simpl.
-          intros HH. contradiction HH.
-          destruct k;  try solve [intros HH;inversion HH].
-          destruct (perm_of_sh sh); auto.
-          intros HH;inversion HH.
-          intros HH;inversion HH.
+          destruct (perm_of_res (r @ (b, ofs))); done.
       Qed.
 
     Definition juicyRestrict {phi:rmap}{m:Mem.mem}(coh:access_cohere' m phi): Mem.mem:=
@@ -616,13 +640,13 @@ Qed.
     Lemma juicyRestrictContentCoh: forall phi m (coh:access_cohere' m phi) (ccoh:contents_cohere m phi),
         contents_cohere (juicyRestrict coh) phi.
     Proof.
-      unfold contents_cohere; intros. rewrite <- juicyRestrictContents.
+      unfold contents_cohere, juicy_mem.contents_cohere; intros. rewrite <- juicyRestrictContents.
       eapply ccoh; eauto.
     Qed.
     Lemma juicyRestrictMaxCoh: forall phi m (coh:access_cohere' m phi) (ccoh:max_access_cohere m phi),
         max_access_cohere (juicyRestrict coh) phi.
     Proof.
-      unfold max_access_cohere; intros.
+      unfold max_access_cohere, juicy_mem.max_access_cohere; intros.
       repeat rewrite <- juicyRestrictMax.
       repeat rewrite <- juicyRestrictNextblock.
       apply ccoh.
@@ -642,7 +666,7 @@ Qed.
     Proof.
       intros. unfold juicyRestrict.
       unfold access_at.
-      destruct (restrPermMap_correct (juice2Perm_cohere coh) loc#1 loc#2) as [MAX CUR].
+      destruct (restrPermMap_correct (juice2Perm_cohere coh) loc.1 loc.2) as [MAX CUR].
       unfold permission_at in *.
       rewrite CUR.
       unfold juice2Perm.
@@ -650,12 +674,12 @@ Qed.
       unfold PMap.get.
       rewrite PTree.gmap; simpl.
       destruct ((PTree.map1
-             (fun f : Z -> perm_kind -> option permission => f^~ Max)
-             (Mem.mem_access m)#2) ! (loc#1)) as [VALUE|]  eqn:THING.
+             (fun f ofs => f ofs Max)
+             (Mem.mem_access m).2) !! (loc.1)) as [VALUE|]  eqn:THING.
       - destruct loc; simpl.
         destruct ((perm_of_res (phi @ (b, z)))) eqn:HH; rewrite HH; reflexivity.
       - simpl. rewrite PTree.gmap1 in THING.
-        destruct (((Mem.mem_access m)#2) ! (loc#1)) eqn:HHH; simpl in THING; try solve[inversion THING].
+        destruct (((Mem.mem_access m).2) !! (loc.1)) eqn:HHH; simpl in THING; try solve[inversion THING].
         unfold access_cohere' in coh.
         unfold max_access_at, access_at in coh. unfold PMap.get in coh.
         generalize (coh loc).
@@ -669,23 +693,21 @@ Qed.
     Lemma juicyRestrictAccCoh: forall phi m (coh:access_cohere' m phi),
         access_cohere (juicyRestrict coh) phi.
     Proof.
-      unfold access_cohere; intros.
+      unfold access_cohere, juicy_mem.access_cohere; intros.
       rewrite juicyRestrictCurEq.
-      destruct ((perm_of_res (phi @ loc))) eqn:HH; try rewrite HH; simpl; reflexivity.
+      apply perm_order''_refl.
     Qed.
 
     Lemma po_perm_of_res: forall r,
-       Mem.perm_order''  (perm_of_res' r) (perm_of_res r).
+       Mem.perm_order'' (perm_of_res' r) (perm_of_res r).
     Proof.
-      rewrite /perm_of_res /perm_of_res' => r.
-      destruct r; try solve[ apply po_refl].
-      assert (Mem.perm_order'' (perm_of_sh sh) (Some Nonempty)).
-      { destruct (perm_of_sh sh) eqn:HH; try solve[constructor].
-        apply perm_of_empty_inv in HH; subst sh.
-        exfalso; apply shares.bot_unreadable; eauto. }
-      destruct k; first[ apply po_refl | assumption].
+      rewrite /perm_of_res'; intros (d, r).
+      destruct (perm_of_res_cases d r) as [(? & ? & ->) | (? & ->)]; first apply po_refl.
+      if_tac; first apply po_None.
+      if_tac; first apply po_None.
+      simpl; destruct (perm_of_dfrac d) eqn:HH; try solve [constructor].
+      apply perm_of_dfrac_None in HH as [-> | ->]; done.
     Qed.
-
 
     Lemma max_acc_coh_acc_coh: forall m phi,
         max_access_cohere m phi -> access_cohere' m phi.
@@ -702,210 +724,12 @@ Qed.
     Lemma juicyRestrictAccCoh': forall phi m (coh:max_access_cohere m phi),
         access_cohere (juicyRestrict' coh) phi.
     Proof.
-      unfold access_cohere; intros.
+      unfold access_cohere, juicy_mem.access_cohere; intros.
       rewrite juicyRestrictCurEq.
-      destruct ((perm_of_res (phi @ loc))) eqn:HH; try rewrite HH; simpl; reflexivity.
+      apply po_refl.
     Qed.
 
-    (*Move this to veric.juicy_mem_lemmas.v *)
-    Lemma po_join_sub': forall r1 r2 : resource,
-        join_sub r2 r1 ->
-        Mem.perm_order'' (perm_of_res' r1) (perm_of_res' r2).
-
-      intros r1 r2[r J]; inversion J; subst; simpl.
-      - if_tac.
-        + subst.
-          if_tac.
-          * eauto with *.
-          * apply join_to_bot_l in RJ; subst;
-              congruence.
-        + if_tac; constructor.
-      - destruct k; try solve [constructor].
-        + apply po_join_sub_sh.
-          eexists; eauto.
-        + apply po_join_sub_sh.
-          * eexists; eauto.
-        + apply po_join_sub_sh.
-          * eexists; eauto.
-      - destruct k.
-        + if_tac.
-          * hnf. destruct (perm_of_sh _); apply I.
-          * apply perm_order''_trans with (perm_of_sh sh3).
-            -- apply po_join_sub_sh.
-               ++ eexists; eauto.
-            -- destruct  (perm_of_sh sh3) eqn:E.
-               ++ constructor.
-               ++ pose proof @perm_of_empty_inv _ E; subst.
-                  apply join_to_bot_l in RJ; subst; congruence.
-        + if_tac.
-          * hnf. destruct (perm_of_sh _); apply I.
-          * apply perm_order''_trans with (perm_of_sh sh1).
-            -- apply po_join_sub_sh.
-               ++ eexists; eauto.
-            -- destruct  (perm_of_sh sh1) eqn:E.
-               ++ constructor.
-               ++ pose proof @perm_of_empty_inv _ E; subst; congruence.
-        + if_tac.
-          * hnf. destruct (perm_of_sh _); apply I.
-          * apply perm_order''_trans with (perm_of_sh sh1).
-            -- apply po_join_sub_sh.
-               ++ eexists; eauto.
-            -- destruct  (perm_of_sh sh1) eqn:E.
-               ++ constructor.
-               ++ pose proof @perm_of_empty_inv _ E; subst; congruence.
-      - destruct k; try constructor.
-        + apply po_join_sub_sh; eexists; eauto.
-        + apply po_join_sub_sh; eexists; eauto.
-        + apply po_join_sub_sh; eexists; eauto.
-      - constructor.
-    Qed.
-
-    Lemma mem_access_coh_sub: forall phi1 phi2 m,
-        max_access_cohere m phi1 ->
-        join_sub phi2 phi1 ->
-        max_access_cohere m phi2.
-    Proof.
-      rewrite /max_access_cohere => phi1 phi2 m H H0 loc.
-      eapply po_trans; eauto.
-      eapply po_join_sub'.
-      apply resource_at_join_sub; assumption.
-    Qed.
-
-    Lemma mem_cohere_sub: forall phi1 phi2 m,
-        mem_cohere' m phi1 ->
-        join_sub phi2 phi1 ->
-        mem_cohere' m phi2.
-    Proof.
-      intros. constructor.
-      - unfold contents_cohere; intros.
-        eapply resource_at_join_sub with (l:= loc) in H0.
-        rewrite H1 in H0.
-        inversion H; clear - H0 cont_coh0.
-        destruct H0 as [X H0].
-        inversion H0; subst.
-        + symmetry in H. apply cont_coh0 in H; assumption.
-        + symmetry in H; apply cont_coh0 in H; assumption.
-      (* - intros loc.
-        eapply resource_at_join_sub with (l:= loc) in H0.
-        eapply po_join_sub  in H0.
-        eapply po_trans; eauto.
-        inversion H; auto. *)
-      - inversion H.
-        eapply mem_access_coh_sub; eauto.
-      - unfold alloc_cohere.
-        inversion H. clear - H0 all_coh0.
-        intros loc HH; apply all_coh0 in HH.
-        apply resource_at_join_sub with (l:= loc) in H0.
-        rewrite HH in H0.
-        destruct H0 as [X H0].
-        inversion H0; auto.
-        apply split_identity in RJ; auto.
-        apply identity_share_bot in RJ; subst; auto.
-        f_equal; apply proof_irr.
-    Qed.
-
-    
-    Lemma join_threads_sub:
-      forall js i (cnt:containsThread js i) r0
-        (H0:join_threads js r0),
-        join_sub (getThreadR cnt) r0.
-    Proof.
-      intros.
-      
-      unfold getThreadR. unfold join_threads in H0.
-      unfold getThreadsR in H0.
-      destruct js; simpl in *.
-      pose proof (mem_ord_enum (n:= n num_threads0)).
-
-      specialize (H (Ordinal (n:=n num_threads0) (m:=i) cnt)) .
-      unfold join_list in H0.
-
-      simpl in H0.
-
-
-      replace (enums_equality.enum num_threads0) with (ord_enum (n num_threads0)) in H0.
-      forget (ord_enum (n num_threads0)) as el.
-      forget ((Ordinal (n:=n num_threads0) (m:=i) cnt)) as j.
-      revert H H0; clear; revert r0; induction el; intros. inv H.
-      unfold in_mem in H. unfold pred_of_mem in H. simpl in H.
-      pose proof @orP.
-      specialize (H1 (j == a)(mem_seq (T:=ordinal_eqType (n num_threads0)) el j)).
-      destruct ((j == a)
-                || mem_seq (T:=ordinal_eqType (n num_threads0)) el j); inv H.
-      inv H1. destruct H.
-      pose proof (@eqP _ j a). destruct (j==a); inv H; inv H1.
-      simpl in H0. destruct H0 as [? [? ?]].
-      exists x; auto.
-      unfold mem_seq in H.
-      destruct H0 as [? [? ?]].
-      apply (IHel x) in H; auto. apply join_sub_trans with x; auto. eexists; eauto.
-      apply ord_enum_enum.
-    Qed.
-
-    Lemma compatible_threadRes_sub:
-      forall js i (cnt:containsThread js i),
-      forall all_juice,
-        join_all js all_juice ->
-        join_sub (getThreadR cnt) all_juice.
-    Proof.
-      intros. inv H.
-      assert (H9: join_sub (Some (getThreadR cnt)) (Some all_juice));
-        [ | destruct H9 as [x H9]; inv H9; [apply join_sub_refl | eexists; eauto]].
-      apply join_sub_trans with (Some r2); [ | eexists; constructor; eauto].
-      apply join_sub_trans with (Some r0); [ | eexists; eauto].
-      clear - H0.
-      assert (H9: join_sub (getThreadR cnt) r0) by (eapply join_threads_sub; eauto).
-      destruct H9 as [x H9]; exists (Some x); constructor; auto.
-    Qed.
-
-    Lemma join_sub_souble_join:
-      forall (a1 b1 c1 a2 b2 c2: rmap),
-        join_sub a1 a2 ->
-        join_sub b1 b2 ->
-        sepalg.join a1 b1 c1 ->
-        sepalg.join a2 b2 c2 ->
-        join_sub c1 c2.
-    Proof.
-      intros.  
-      inv H. inv H0.
-      eapply sepalg.join_comm in H3.
-      pose proof (sepalg.join_assoc H3 H2) as X.
-      destruct X as (x1 & ? & ?).
-      eapply sepalg.join_comm in H.
-      eapply sepalg.join_comm in H0.
-      pose proof (sepalg.join_assoc H H0) as X.
-      destruct X as (x2 & ? & ?).
-      eapply sepalg.join_comm in H5.
-      eapply sepalg.join_comm in H4.
-      eapply sepalg.join_comm in H6.
-      pose proof (sepalg.join_assoc H6 H4) as X.
-      destruct X as (x3 & ? & ?).
-      exists x3.
-      replace c1 with x2; auto.
-      eapply sepalg.join_eq; auto.
-    Qed.
-
-    Lemma join_list_not_none:
-      forall el l phi x,
-        join_list' (List.map snd el) x ->
-        SetoidList.InA (AMap.eq_key_elt (elt:=option rmap))
-                       (l, Some phi) el ->
-        exists s, x = Some s.
-    Proof.
-      induction el.
-      - intros. inv H0.
-      - intros. destruct H as (?&?&?).
-        inv H0.
-        + inv H3. simpl in *.
-          replace a.2 with (Some phi) in H;
-            inv H;
-            eexists; reflexivity.
-        + exploit IHel; eauto.
-          intros [s HH].
-          subst x0. inv H; eexists; reflexivity.
-    Qed.
-    
-    Lemma compatible_lockRes_sub:
+(*    Lemma compatible_lockRes_sub:
       forall js l (phi:rmap) all_juice,
         join_locks js (Some all_juice) ->
         lockRes(resources:=LocksAndResources) js l = Some (Some phi) ->
@@ -934,7 +758,7 @@ Qed.
           * eapply join_sub_trans.
             eapply IHel; eauto.
             eexists; eauto.
-    Qed.
+    Qed.*)
     Lemma lockres_join_locks_not_none:
       forall js a d_phi,
         lockRes(resources:=LocksAndResources)
@@ -944,27 +768,70 @@ Qed.
       intros.
       apply AMap.find_2 in H. unfold OrdinalPool.lockGuts in *.
       apply AMap.elements_1 in H. simpl in *.
-      intros HH. 
+      intros HH.
       unfold join_locks in HH.
-      exploit join_list_not_none; eauto.
-      intros [? ?]; discriminate.
-    Qed.
-    Lemma lock_thread_sub_all_juice:
-      forall js all_juice d_phi phi i Hi a,
-        join_all js all_juice ->
-        lockRes js a = Some (Some d_phi) ->
-        sepalg.join (@getThreadR _ _ _ i js Hi) d_phi phi ->
-        join_sub phi all_juice.
-    Proof.
-      intros.
-      inv H. inv H4.
-      - exfalso; eapply lockres_join_locks_not_none; eauto.
-      - eapply join_sub_trans; [|eexists; eauto].
-        eapply join_sub_souble_join; eauto.
-        eapply join_threads_sub; assumption.
-        eapply compatible_lockRes_sub; eassumption.
+      symmetry in HH; rewrite None_equiv_eq in HH.
+      eapply join_list_not_none in HH; first done.
+      apply SetoidList.InA_alt in H as ((?, ?) & (? & ?) & ?); simpl in *; subst.
+      rewrite in_map_iff; eexists (_, _); simpl; eauto.
     Qed.
 
+    Lemma mem_cohere_sub: forall (phi1 phi2 : rmap) m, ✓ phi1 ->
+        mem_cohere' m phi1 ->
+        phi2 ≼ phi1 ->
+        mem_cohere' m phi2.
+    Proof.
+      intros ??? Hv [???] H; split.
+      - intros loc.
+        rewrite gmap.lookup_included in H; specialize (H loc).
+        eapply contents_cohere_mono, cont_coh0.
+        by apply resR_le.
+      - intros loc.
+        rewrite gmap.lookup_included in H; specialize (H loc).
+        assert (✓ (phi1 !! loc))%stdpp by done.
+        eapply max_access_cohere_mono, max_coh0; last by apply resR_le.
+        rewrite resR_to_resource_fst; destruct (phi1 !! loc)%stdpp eqn: Hl; rewrite Hl in H0 |- *; try done.
+        by apply dfrac_of'_valid.
+      - intros ? Hout; specialize (all_coh0 _ Hout).
+        rewrite gmap.lookup_included in H; specialize (H loc).
+        apply option_included in H as [? | (? & ? & H1 & ? & ?)]; try done.
+        rewrite all_coh0 // in H.
+    Qed.
+
+    Lemma join_threads_sub:
+      forall js i (cnt:containsThread js i) r0
+        (H0:join_threads js r0),
+        getThreadR cnt ≼ r0.
+    Proof.
+      intros.
+      unfold getThreadR. unfold join_threads in H0.
+      unfold getThreadsR in H0.
+      destruct js; simpl in *.
+      pose proof (fintype.mem_ord_enum (n:= n num_threads0) (fintype.Ordinal (n:=n num_threads0) (m:=i) cnt)) as H.
+      rewrite -ord_enum_enum in H0.
+      eapply (cmra_included_proper(A := resource_map.rmapUR _ _)); [done | apply H0 |].
+      edestruct (big_opL_In id (map perm_maps0 (fintype.ord_enum (n num_threads0))) (perm_maps0 (fintype.Ordinal (n:=n num_threads0) (m:=i) cnt))) as (x & ->); last by eexists.
+      rewrite in_map_iff; eexists; split; first done.
+      clear - H.
+      forget (fintype.ord_enum (n num_threads0)) as el.
+      forget (fintype.Ordinal (n:=n num_threads0) (m:=i) cnt) as j.
+      clear - H; induction el; simpl in *; try done.
+      unfold in_mem in H. unfold pred_of_mem in H. simpl in H.
+      destruct (@eqtype.eqP (fintype.ordinal_eqType (n num_threads0)) j a); auto.
+    Qed.
+
+    Lemma compatible_threadRes_sub:
+      forall js i (cnt:containsThread js i),
+      forall all_juice,
+        join_all js all_juice ->
+        (getThreadR cnt) ≼ all_juice.
+    Proof.
+      intros. inv H.
+      rewrite -(Some_included_total(A := resource_map.rmapUR _ _)).
+      rewrite -H3 Some_op -H2.
+      etrans; first by apply Some_included_2, join_threads_sub.
+      rewrite -assoc; by eexists.
+    Qed.
 
     Lemma mem_compat_thread_max_cohere {tp m} (compat: mem_compatible tp m):
       forall {i} cnti,
@@ -973,11 +840,17 @@ Qed.
       destruct compat as [x compat] => i cnti loc.
       apply po_trans with (b:= perm_of_res' (x @ loc)).
       - inversion compat. inversion all_cohere0. apply max_coh0.
-      - (*This comes from *)
-        apply po_join_sub'.
-        apply resource_at_join_sub.
-        eapply compatible_threadRes_sub.
-        inversion compat; inversion all_cohere0; assumption.
+      - pose proof (mem_compatible_with_valid compat) as Hv.
+        specialize (Hv loc).
+        apply perm_of_dfrac_mono.
+        { rewrite /resource_at resR_to_resource_fst.
+          destruct (_ !! _)%stdpp; last done.
+          by apply dfrac_of'_valid. }
+        inv compat.
+        apply (compatible_threadRes_sub cnti) in juice_join0.
+        rewrite gmap.lookup_included in juice_join0.
+        specialize (juice_join0 loc).
+        apply resR_le in juice_join0 as (? & ?); done.
     Qed.
 
     Lemma thread_mem_compatible: forall tp m,
@@ -986,31 +859,35 @@ Qed.
     Proof. intros. destruct H as [allj H].
            inversion H.
            unfold mem_thcohere; intros.
+           assert (✓ allj) by (inv juice_join0; done).
            eapply compatible_threadRes_sub  with (cnt:=cnt)in juice_join0.
            eapply mem_cohere_sub; eauto.
     Qed.
 
-    Lemma compatible_lockRes_sub_all: forall js l phi,
-        lockRes js l = Some (Some phi) ->
+    Lemma join_locks_sub: forall js l phi r0
+        (Hl : lockRes js l = Some (Some phi)) (H0 : join_locks js r0),
+        Some phi ≼ r0.
+    Proof.
+      intros.
+      eapply (cmra_included_proper(A := optionR _)); [done..|].
+      apply AMap.find_2 in Hl. unfold OrdinalPool.lockGuts in *.
+      apply AMap.elements_1 in Hl.
+      apply SetoidList.InA_alt in Hl as ((?, ?) & (? & ?) & ?); simpl in *; subst.
+      edestruct (big_opL_In(o := op(A := optionR _)) id (map snd (AMap.elements (elt:=option rmap) (lset js))) (Some phi)) as (x & ->); last by eexists.
+      rewrite in_map_iff; eexists (_, _); simpl; eauto.
+    Qed.
+
+    Lemma compatible_lockRes_sub_all: forall js l phi
+        (Hl : lockRes js l = Some (Some phi)),
         forall all_juice,
           join_all js all_juice ->
-          join_sub phi all_juice.
+          phi ≼ all_juice.
     Proof.
-     intros.
-     inv H0.
-     eapply join_sub_trans; [|eexists; eauto].
-     assert (H9: join_sub (Some phi) (Some r2));
-       [ | destruct H9 as [x H9]; inv H9; [apply join_sub_refl | eexists; eauto]].
-     apply join_sub_trans with (b:=r1); [ | eexists; eauto].
-     clear - H H2.
-     hnf in H2. simpl in H. simpl in *.
-     apply AMap.find_2 in H. unfold OrdinalPool.lockGuts in H.
-     apply AMap.elements_1 in H. simpl in *.
-     forget (AMap.elements (elt:= option rmap) (lset js)) as el.
-     revert r1 H2; induction el; simpl; intros. inv H.
-     destruct H2 as [? [? ?]]. destruct a; simpl in *. inv H. inv H3. simpl in *; subst.
-     exists x; auto. apply IHel in H1; auto.
-     apply join_sub_trans with x; auto. exists o; auto.
+     intros. inv H.
+     rewrite -(Some_included_total(A := resource_map.rmapUR _ _)).
+     rewrite -H3 Some_op -H2.
+     etrans; first by eapply join_locks_sub.
+     rewrite (cmra_comm(A := optionR _) _ r1) -assoc; by eexists.
    Qed.
 
     Lemma lock_mem_compatible: forall tp m,
@@ -1019,36 +896,31 @@ Qed.
     Proof. intros.  destruct H as [allj H].
            inversion H.
            unfold mem_thcohere; intros.
-          unfold mem_lock_cohere; intros.
-          eapply compatible_lockRes_sub_all in juice_join0; [|apply H0].
-          eapply mem_cohere_sub; eauto.
+           unfold mem_lock_cohere; intros.
+           assert (✓ allj) by (inv juice_join0; done).
+           eapply compatible_lockRes_sub_all in juice_join0; [|apply H0].
+           eapply mem_cohere_sub; eauto.
     Qed.
 
 
     (* PERSONAL MEM: Is the contents of the global memory,
-       with the juice of a single thread and the Cur that corresponds to that juice.*)
-    Definition acc_coh:= fun m phi pr => @max_acc_coh_acc_coh m phi (max_coh pr).
-    Definition personal_mem {m phi} (pr : mem_cohere' m phi) : juicy_mem:=
-      mkJuicyMem
-        (@juicyRestrict phi m (acc_coh pr))
-        phi
-        (juicyRestrictContentCoh (acc_coh pr) (cont_coh pr))
-        (juicyRestrictAccCoh (acc_coh pr))
-        (juicyRestrictMaxCoh (acc_coh pr) (max_coh pr))
-        (juicyRestrictAllocCoh (acc_coh pr) (all_coh pr)).
+       with the Cur permissions of one thread's rmap.*)
+    Definition acc_coh := fun m phi pr => @max_acc_coh_acc_coh m phi (max_coh pr).
+    Definition personal_mem {m phi} (pr : mem_cohere' m phi) : mem :=
+        (@juicyRestrict phi m (acc_coh pr)).
 
-    Definition juicy_sem := (FSem.F _ _ JuicyFSem.t) _ the_sem.
+    (*Definition juicy_sem := (FSem.F _ _ JuicyFSem.t) _ the_sem.*)
     (* Definition juicy_step := (FSem.step _ _ JuicyFSem.t) _ _ the_sem. *)
 
     Program Definition first_phi (tp : thread_pool) : rmap := (@getThreadR _ _ _ 0%nat tp _).
     Next Obligation.
-      unfold OrdinalPool.containsThread.
-      destruct num_threads.
-      simpl.
-      ssrlia.
+      intros tp.
+      hnf.
+      destruct num_threads; simpl.
+      apply /ssrnat.leP; lia.
     Defined.
 
-    Program Definition level_tp (tp : thread_pool) := level (first_phi tp).
+(*    Program Definition level_tp (tp : thread_pool) := level (first_phi tp).
 
     Definition tp_level_is_above n tp :=
       (forall i (cnti : containsThread tp i), le n (level (getThreadR cnti))) /\
@@ -1058,7 +930,7 @@ Qed.
     Definition tp_level_is n tp :=
       (forall i (cnti : containsThread tp i), level (getThreadR cnti) = n) /\
       (forall i phi, lockRes(resources:=LocksAndResources) tp i = Some (Some phi) -> level phi = n) /\
-      n = level (extraRes tp).
+      n = level (extraRes tp).*)
 
     (*
     Lemma mem_compatible_same_level tp m :
@@ -1084,7 +956,7 @@ Qed.
         eapply (DLT _); eauto.
     Qed. *)
 
-    Definition cnt_from_ordinal tp : forall i : ordinal (pos.n (num_threads tp)), containsThread tp i.
+(*    Definition cnt_from_ordinal tp : forall i : fintype.ordinal (pos.n (num_threads tp)), OrdinalPool.containsThread tp i.
       intros [i pr]; apply pr. Defined.
 
     Definition age_tp_to (k : nat) (tp : thread_pool) : thread_pool :=
@@ -1236,7 +1108,7 @@ Qed.
       destruct js; auto.
     Qed.
 
-    Lemma cnt_age' {js i age} :
+    Lemma {js i age} :
         containsThread js i ->
         containsThread (age_tp_to age js) i.
     Proof.
@@ -1251,25 +1123,23 @@ Qed.
       destruct tp; simpl.
       f_equal. f_equal.
       apply cnt_irr.
-    Qed.
+    Qed.*)
 
     Inductive juicy_step  {tid0 tp m} (cnt: containsThread tp tid0)
       (Hcompatible: mem_compatible tp m) : thread_pool -> mem -> list mem_event -> Prop :=
     | step_juicy :
-        forall (tp':thread_pool) c jm jm' m' (c' : C),
+        forall (tp':thread_pool) c m1 phi' m' (c' : C),
           forall (Hpersonal_perm:
-               personal_mem (thread_mem_compatible Hcompatible cnt) = jm)
+               personal_mem (thread_mem_compatible Hcompatible cnt) = m1)
             (Hinv : invariant tp)
             (Hthread: getThreadC cnt = Krun c)
-            (Hcorestep: corestep juicy_sem c jm c' jm')
-            (Htp': tp' = @updThread _ _ _ tid0 (age_tp_to (level jm') tp) (cnt_age' cnt) (Krun c') (m_phi jm'))
-            (Hm': m_dry jm' = m'),
-            juicy_step  cnt Hcompatible tp' m' [::].
+            (Hcorestep: corestep the_sem c m1 c' m')
+            (Htp': tp' = @updThread _ _ _ tid0 tp cnt (Krun c') phi') (* can we leave phi' unconstrained? *),
+            juicy_step  cnt Hcompatible tp' m' nil.
 
-    Definition pack_res_inv (R: pred rmap) := SomeP rmaps.Mpred (fun _ => R) .
-  
-    Definition lock_at_least sh R phi b ofs :=
-          forall i, 0 <= i < LKSIZE -> exists sh' rsh', join_sub sh sh' /\ phi@(b,ofs+i) = YES sh' rsh' (LK LKSIZE i) (pack_res_inv R).
+    (* Trying without tracking lock invariants. *)
+    Definition lock_at_least (sh : dfrac) (phi : rmap) b ofs :=
+          forall i, 0 <= i < LKSIZE -> exists sh', sh ≼ sh' /\ (phi @ (b,ofs+i))%stdpp = (sh', Some (LK LKSIZE i)).
 
 
     Notation Kblocked := (threadPool.Kblocked).
@@ -1278,7 +1148,7 @@ Qed.
               (cnt0:containsThread tp tid0)(Hcompat:mem_compatible tp m):
       thread_pool -> mem -> sync_event -> Prop :=
     | step_acquire :
-        forall (tp' tp'' tp''':thread_pool) c m0 m1 b ofs d_phi phi phi' m' pmap_tid',
+        forall (tp' tp'':thread_pool) c m0 m1 b ofs d_phi phi phi' m' pmap_tid',
           forall
             (Hinv : invariant tp)
             (Hthread: getThreadC cnt0 = Kblocked c)
@@ -1287,8 +1157,8 @@ Qed.
             (*Hpersonal_perm:
                personal_mem cnt0 Hcompatible = jm*)
             (Hpersonal_juice: getThreadR cnt0 = phi)
-            (sh:Share.t)(R:pred rmap)
-            (HJcanwrite: lock_at_least sh R phi b (Ptrofs.intval ofs))
+            sh
+            (HJcanwrite: lock_at_least sh phi b (Ptrofs.intval ofs))
             (Hrestrict_map0: juicyRestrict_locks
                               (mem_compat_thread_max_cohere Hcompat cnt0) = m0)
             (Hload: Mem.load Mptr m0 b (Ptrofs.intval ofs) = Some (Vptrofs Ptrofs.one))
@@ -1304,13 +1174,12 @@ Qed.
             (Hrestrict_pmap: restrPermMap Hlt' = m1)
             (Hstore: Mem.store Mptr m1 b (Ptrofs.intval ofs) (Vptrofs Ptrofs.zero) = Some m')
             (His_unlocked: lockRes tp (b, Ptrofs.intval ofs) = SSome d_phi)
-            (Hadd_lock_res: join phi d_phi phi')
+            (Hadd_lock_res: phi' = phi ⋅ d_phi)
             (Htp': tp' = updThread cnt0 (Kresume c Vundef) phi')
-            (Htp'': tp'' = updLockSet tp' (b, Ptrofs.intval ofs) None )
-            (Htp''': tp''' = age_tp_to (level phi - 1)%nat tp''),
-            syncStep' cnt0 Hcompat tp''' m' (acquire (b, Ptrofs.intval ofs) None)
+            (Htp'': tp'' = updLockSet tp' (b, Ptrofs.intval ofs) None),
+            syncStep' cnt0 Hcompat tp'' m' (acquire (b, Ptrofs.intval ofs) None)
     | step_release :
-        forall  (tp' tp'' tp''':thread_pool) c m0 m1 b ofs  (phi d_phi :rmap) (R: pred rmap) phi' m' pmap_tid',
+        forall  (tp' tp'':thread_pool) c m0 m1 b ofs  (phi d_phi :rmap) phi' m' pmap_tid',
           forall
             (Hinv : invariant tp)
             (Hthread: getThreadC cnt0 = Kblocked c)
@@ -1319,8 +1188,8 @@ Qed.
             (* Hpersonal_perm:
                personal_mem cnt0 Hcompatible = jm *)
             (Hpersonal_juice: getThreadR cnt0 = phi)
-            (sh:Share.t) 
-            (HJcanwrite: lock_at_least sh R phi b (Ptrofs.intval ofs))
+            sh 
+            (HJcanwrite: lock_at_least sh phi b (Ptrofs.intval ofs))
             (Hrestrict_map0: juicyRestrict_locks
                               (mem_compat_thread_max_cohere Hcompat cnt0) = m0)
             (Hload: Mem.load Mptr m0 b (Ptrofs.intval ofs) = Some (Vptrofs Ptrofs.zero))
@@ -1336,15 +1205,13 @@ Qed.
             (Hrestrict_pmap: restrPermMap Hlt' = m1)
             (Hstore: Mem.store Mptr m1 b (Ptrofs.intval ofs) (Vptrofs Ptrofs.one) = Some m')
             (His_locked: lockRes tp (b, Ptrofs.intval ofs) = SNone )
-            (Hsat_lock_inv: R (age_by 1 d_phi))
-            (Hrem_lock_res: join d_phi phi' phi)
+            (Hrem_lock_res: phi = d_phi ⋅ phi')
             (Htp': tp' = updThread cnt0 (Kresume c Vundef) phi')
             (Htp'': tp'' =
-                    updLockSet tp' (b, Ptrofs.intval ofs) (Some d_phi))
-            (Htp''': tp''' = age_tp_to (level phi - 1)%nat tp''),
-            syncStep' cnt0 Hcompat tp''' m' (release (b, Ptrofs.intval ofs) None)
+                    updLockSet tp' (b, Ptrofs.intval ofs) (Some d_phi)),
+            syncStep' cnt0 Hcompat tp'' m' (release (b, Ptrofs.intval ofs) None)
     | step_create :
-        forall  (tp_upd tp':thread_pool) c vf arg jm (d_phi phi': rmap) b ofs (* P Q *),
+        forall  (tp_upd tp':thread_pool) c vf arg (d_phi phi': rmap) b ofs (* P Q *),
           forall
             (Hinv : invariant tp)
             (Hthread: getThreadC cnt0 = Kblocked c)
@@ -1352,15 +1219,12 @@ Qed.
                            Some (CREATE, vf::arg::nil))
 (*            (Harg: Val.inject (Mem.flat_inj (Mem.nextblock m)) arg arg) *)
             (Hfun_sepc: vf = Vptr b ofs)
-            (Hpersonal_perm:
-               personal_mem (thread_mem_compatible Hcompat cnt0) = jm)
-            (Hrem_fun_res: join d_phi phi' (m_phi jm))
+            (Hrem_fun_res: getThreadR cnt0 = d_phi ⋅ phi')
             (Htp': tp_upd = updThread cnt0 (Kresume c Vundef) phi')
-            (Htp'': tp' = age_tp_to (level (m_phi jm) - 1)%nat (addThread tp_upd vf arg d_phi)),
+            (Htp'': tp' = addThread tp_upd vf arg d_phi),
             syncStep' cnt0 Hcompat tp' m (spawn (b, Ptrofs.intval ofs) None None)
     | step_mklock :
-        forall  (tp' tp'': thread_pool)  jm c b ofs R ,
-          let: phi := m_phi jm in
+        forall  (tp' tp'': thread_pool) m c b ofs,
           forall
             phi' m'
             (Hinv : invariant tp)
@@ -1369,23 +1233,21 @@ Qed.
                            Some (MKLOCK, Vptr b ofs::nil))
             (*Hright_juice:  m = m_dry jm*)
             (Hpersonal_perm:
-               personal_mem (thread_mem_compatible Hcompat cnt0) = jm)
-            (Hpersonal_juice: getThreadR cnt0 = phi)
+               personal_mem (thread_mem_compatible Hcompat cnt0) = m)
             (*Check I have the right permission to mklock and the right value (i.e. 0) *)
             (*Haccess: address_mapsto LKCHUNK (Vint Int.zero) sh Share.top (b, Ptrofs.intval ofs) phi*)
             (Hstore:
-               Mem.store Mptr (m_dry jm) b (Ptrofs.intval ofs) (Vptrofs Ptrofs.zero) = Some m')
+               Mem.store Mptr m b (Ptrofs.intval ofs) (Vptrofs Ptrofs.zero) = Some m')
             (* [Hrmap] replaced: [Hct], [Hlock], [Hj_forward] and [levphi'].
                This says that phi and phi' coincide everywhere except in adr_range,
                and specifies how phi and phi' should differ in adr_range
                (in particular, they have equal shares, pointwise) *)
-            (Hrmap : rmap_makelock phi phi' (b, Ptrofs.unsigned ofs) R LKSIZE)
+            (Hrmap : rmap_makelock (getThreadR cnt0) phi' (b, Ptrofs.unsigned ofs) LKSIZE)
             (Htp': tp' = updThread cnt0 (Kresume c Vundef) phi')
-            (Htp'': tp'' = age_tp_to (level phi - 1)%nat
-                    (updLockSet tp' (b, Ptrofs.intval ofs) None )),
+            (Htp'': tp'' = updLockSet tp' (b, Ptrofs.intval ofs) None),
             syncStep' cnt0 Hcompat tp'' m' (mklock (b, Ptrofs.intval ofs))
     | step_freelock :
-        forall  (tp' tp'': thread_pool) c b ofs phi R phi',
+        forall  (tp' tp'': thread_pool) c b ofs phi phi',
           forall
             (Hinv : invariant tp)
             (Hthread: getThreadC cnt0 = Kblocked c)
@@ -1395,26 +1257,22 @@ Qed.
             (*First check the lock is acquired:*)
             (His_acq: lockRes tp (b, (Ptrofs.intval ofs)) = SNone)
             (*Relation between rmaps:*)
-            (Hrmap : rmap_freelock phi phi' m (b, Ptrofs.unsigned ofs) R LKSIZE)
+            (Hrmap : rmap_freelock phi phi' m (b, Ptrofs.unsigned ofs) LKSIZE)
             (Htp': tp' = updThread cnt0 (Kresume c Vundef) phi')
-            (Htp'': tp'' = age_tp_to (level phi - 1)%nat
-                    (remLockSet tp' (b, Ptrofs.intval ofs) )),
+            (Htp'': tp'' = remLockSet tp' (b, Ptrofs.intval ofs)),
             syncStep' cnt0 Hcompat  tp'' m (freelock (b, Ptrofs.intval ofs))
 
     | step_acqfail :
-        forall  c b ofs jm m1,
-          let: phi := m_phi jm in
+        forall c b ofs m1,
           forall
             (Hinv : invariant tp)
             (Hthread: getThreadC cnt0 = Kblocked c)
             (Hat_external: at_external the_sem c m =
                            Some (LOCK, Vptr b ofs::nil))
-            (Hpersonal_perm:
-               personal_mem (thread_mem_compatible Hcompat cnt0) = jm)
             (Hrestrict_map: juicyRestrict_locks
                               (mem_compat_thread_max_cohere Hcompat cnt0) = m1)
-            (sh:Share.t) (R:pred rmap)
-            (HJcanwrite: lock_at_least sh R phi b (Ptrofs.intval ofs))
+            sh
+            (HJcanwrite: lock_at_least sh (getThreadR cnt0) b (Ptrofs.intval ofs))
             (Hload: Mem.load Mptr m1 b (Ptrofs.intval ofs) = Some (Vptrofs Ptrofs.zero)),
             syncStep' cnt0 Hcompat tp m (failacq (b,Ptrofs.intval ofs)).
 
@@ -1445,23 +1303,17 @@ Qed.
       - intros [cntj [ q running]].
         inversion H; subst.
         assert (cntj':=cntj).
-        eapply cnt_age' in cntj'.
-        eapply (cntUpdate(resources := LocksAndResources) (Krun c') (m_phi jm') (cnt_age' cntj)) in cntj'.
+        eapply (cntUpdate(resources := LocksAndResources) (Krun c') phi' cntj) in cntj'.
         exists cntj'.
         destruct (NatTID.eq_tid_dec i j).
         + subst j; exists c'.
           rewrite gssThreadCode; reflexivity.
         + exists q.
           rewrite gsoThreadCode; auto.
-          generalize running; destruct tp; simpl.
-          intros RUN; rewrite <- RUN.
-          f_equal. f_equal.
-          apply cnt_irr.
       - intros [cntj' [ q' running]].
         inversion H; subst.
         assert (cntj:=cntj').
-        eapply cnt_age in cntj.
-        eapply cntUpdate' with(c:=Krun c')(p:=m_phi jm') in cntj; eauto.
+        eapply cntUpdate' with(c:=Krun c')(p:=phi') in cntj; eauto.
         exists cntj.
         destruct (NatTID.eq_tid_dec i j).
         + subst j; exists c.
@@ -1470,10 +1322,6 @@ Qed.
           apply cnt_irr.
         + exists q'.
           rewrite gsoThreadCode in running; auto.
-          rewrite <- running.
-          destruct tp; simpl.
-          f_equal. f_equal.
-          apply cnt_irr.
     Qed.
 
     Definition syncStep (isCoarse:bool) :
@@ -1501,24 +1349,19 @@ Qed.
           end.
       + (*this should be easy to automate or shorten*)
         inversion H; subst.
-        * exists (cnt_age' (cntUpdateL _ _ (cntUpdate (Kresume c Vundef) phi' _ cntj))), q.
-          erewrite <- age_getThreadCode.
+        * exists ((cntUpdateL _ _ (cntUpdate (Kresume c Vundef) (getThreadR cnt ⋅ d_phi) _ cntj))), q.
           rewrite gLockSetCode.
           rewrite gsoThreadCode; assumption.
-        * exists (cnt_age' (cntUpdateL _ _ (cntUpdate(resources:=LocksAndResources) (Kresume c Vundef) phi' _ cntj))), q.
-          erewrite <- age_getThreadCode.
+        * exists ((cntUpdateL _ _ (cntUpdate(resources:=LocksAndResources) (Kresume c Vundef) phi' _ cntj))), q.
           rewrite gLockSetCode.
           rewrite gsoThreadCode; assumption.
-        * exists (cnt_age' (cntAdd _ _ _ (cntUpdate(resources:=LocksAndResources) (Kresume c Vundef) phi' _ cntj))), q.
-          erewrite <- age_getThreadCode.
+        * exists ((cntAdd _ _ _ (cntUpdate(resources:=LocksAndResources) (Kresume c Vundef) phi' _ cntj))), q.
           erewrite gsoAddCode . (*i? *)
           rewrite gsoThreadCode; assumption.
-        * exists (cnt_age' (cntUpdateL _ _ (cntUpdate(resources:=LocksAndResources) (Kresume c Vundef) phi' _ cntj))), q.
-          erewrite <- age_getThreadCode.
+        * exists ((cntUpdateL _ _ (cntUpdate(resources:=LocksAndResources) (Kresume c Vundef) phi' _ cntj))), q.
           rewrite gLockSetCode.
           rewrite gsoThreadCode; assumption.
-        * exists (cnt_age' (cntRemoveL _ (cntUpdate(resources:=LocksAndResources) (Kresume c Vundef) phi' _ cntj))), q.
-          erewrite <- age_getThreadCode.
+        * exists ((cntRemoveL _ (cntUpdate(resources:=LocksAndResources) (Kresume c Vundef) phi' _ cntj))), q.
           rewrite gRemLockSetCode.
           rewrite gsoThreadCode; assumption.
         * exists cntj, q; assumption.
@@ -1526,14 +1369,12 @@ Qed.
       destruct (NatTID.eq_tid_dec i j).
       + subst j. generalize running; clear running.
         inversion H; subst;
-        try erewrite <- age_getThreadCode;
           try rewrite gLockSetCode;
           try rewrite gRemLockSetCode;
           try rewrite gssThreadCode;
           try solve[intros HH; inversion HH].
         { (*addthread*)
           assert (cntj':=cntj).
-          eapply cnt_age in cntj'.
           eapply cntAdd' in cntj'. destruct cntj' as [ [HH HHH] | HH].
           * erewrite gsoAddCode; eauto.
             subst; rewrite gssThreadCode; intros AA; inversion AA.
@@ -1544,7 +1385,6 @@ Qed.
             rewrite Hthread; intros HH; inversion HH. }
       + generalize running; clear running.
         inversion H; subst;
-        try erewrite <- age_getThreadCode;
           try rewrite gLockSetCode;
           try rewrite gRemLockSetCode;
           try (rewrite gsoThreadCode; [|auto]);
@@ -1555,20 +1395,18 @@ Qed.
         end).
       (*Add thread case*)
         assert (cntj':=cntj).
-        eapply cnt_age in cntj'.
         eapply cntAdd' in cntj'; destruct cntj' as [ [HH HHH] | HH].
         * erewrite gsoAddCode; eauto.
           destruct (NatTID.eq_tid_dec i j);
             [subst; rewrite gssThreadCode; intros AA; inversion AA|].
           rewrite gsoThreadCode; auto.
           exists HH, q; assumption.
-        * erewrite gssAddCode . intros AA; inversion AA.
+        * erewrite gssAddCode. intros AA; inversion AA.
           assumption.
 
 
 
           Unshelve. all: eauto.
-          apply cntAdd. eauto.
   Qed.
 
 
@@ -1602,7 +1440,7 @@ Qed.
 
     Definition init_mach rmap (m:mem) (tp:thread_pool) (m':mem) (v:val) (args:list val) : Prop :=
       exists c, initial_core the_sem 0 m c m' v args /\
-        match rmap with Some rmap => tp = initial_machine rmap c (id_core rmap) | None => False end.
+        match rmap with Some rmap => tp = initial_machine rmap c (core rmap) | None => False end.
 
 
     Section JuicyMachineLemmas.
@@ -1613,19 +1451,26 @@ Qed.
         forall l r,
           ThreadPool.lockRes js l = Some (Some r) ->
           forall b ofs,
-            Mem.perm_order'' ((getMaxPerm m) !! b ofs) (perm_of_res' (r @ (b, ofs))).
+            Mem.perm_order'' (PMap.get b (getMaxPerm m) ofs) (perm_of_res' (r @ (b, ofs))).
       Proof.
         intros. destruct H as [allj H].
         inversion H.
         cut (Mem.perm_order'' (perm_of_res' (allj @ (b,ofs))) (perm_of_res' (r @ (b, ofs)))).
-      {intros AA. eapply po_trans; eauto.
-       inversion all_cohere0.
-       rewrite getMaxPerm_correct.
-       specialize (max_coh0 (b,ofs)).
-       eapply max_coh0. }
-      { apply po_join_sub'.
-        apply resource_at_join_sub.
-        eapply compatible_lockRes_sub_all; eauto; apply H0. }
+      { intros AA. eapply po_trans; eauto.
+        inversion all_cohere0.
+        rewrite getMaxPerm_correct.
+        specialize (max_coh0 (b,ofs)).
+        eapply max_coh0. }
+      { assert (✓ allj) as Hv by (by inv juice_join0).
+        specialize (Hv (b, ofs)).
+        apply perm_of_dfrac_mono; try done.
+        { rewrite /resource_at resR_to_resource_fst.
+          destruct (_ !! _)%stdpp; last done.
+          by apply dfrac_of'_valid. }
+        eapply compatible_lockRes_sub_all in juice_join0; last done.
+        rewrite gmap.lookup_included in juice_join0.
+        specialize (juice_join0 (b, ofs)).
+        apply resR_le in juice_join0 as (? & ?); done. }
       Qed.
 
 
@@ -1634,45 +1479,28 @@ Qed.
              forall l r,
              ThreadPool.lockRes js l = Some (Some r) ->
              forall b ofs,
-               Mem.perm_order'' ((getMaxPerm m) !! b ofs) (perm_of_res (r @ (b, ofs))).
+               Mem.perm_order'' (PMap.get b (getMaxPerm m) ofs) (perm_of_res (r @ (b, ofs))).
     Proof.
       intros. destruct H as [allj H].
       inversion H.
       cut (Mem.perm_order'' (perm_of_res (allj @ (b,ofs))) (perm_of_res (r @ (b, ofs)))).
-      {intros AA. eapply po_trans; eauto.
-       inversion all_cohere0.
-       rewrite getMaxPerm_correct.
-       eapply max_acc_coh_acc_coh in max_coh0.
-       specialize (max_coh0 (b,ofs)).
-       apply max_coh0. }
-      { apply po_join_sub.
-        apply resource_at_join_sub.
-        eapply compatible_lockRes_sub_all; eauto; apply H0. }
+      { intros AA. eapply po_trans; eauto.
+        inversion all_cohere0.
+        rewrite getMaxPerm_correct.
+        eapply max_acc_coh_acc_coh in max_coh0.
+        specialize (max_coh0 (b,ofs)).
+        apply max_coh0. }
+      { assert (✓ allj) as Hv by (by inv juice_join0).
+        specialize (Hv (b, ofs)).
+        eapply perm_of_res_mono', resR_le; try done.
+        { rewrite /resource_at resR_to_resource_fst.
+          destruct (_ !! _)%stdpp; last done.
+          by apply dfrac_of'_valid. }
+        eapply compatible_lockRes_sub_all in juice_join0; last done.
+        rewrite gmap.lookup_included in juice_join0; eauto. }
     Qed.
 
-    Lemma access_cohere_sub': forall phi1 phi2 m,
-        access_cohere' m phi1 ->
-        join_sub phi2 phi1 ->
-        access_cohere' m phi2.
-    Proof.
-      unfold access_cohere'; intros.
-      eapply po_trans.
-        - apply H.
-        - apply po_join_sub.
-          apply resource_at_join_sub; assumption.
-    Qed.
-
-
-
-      Lemma mem_cohere'_juicy_mem jm : mem_cohere' (m_dry jm) (m_phi jm).
-      Proof.
-        destruct jm as [m phi C A M L]; simpl.
-        constructor; auto.
-      Qed.
-
-
-
-      Lemma compatible_threadRes_join:
+(*      Lemma compatible_threadRes_join:
         forall js m,
           mem_compatible js m ->
           forall i (cnti: containsThread js i) j (cntj: containsThread js j),
@@ -1811,17 +1639,18 @@ Qed.
            apply IHel in H1; auto. apply join_sub_trans with x; auto.
            eexists; eauto.
          }
-    Qed.
+    Qed.*)
 
       Lemma compatible_lockRes_cohere: forall js m l phi,
           lockRes js l = Some (Some phi) ->
           mem_compatible js m ->
-          mem_cohere' m phi .
+          mem_cohere' m phi.
       Proof.
         intros.
         inversion H0 as [all_juice M]; inversion M.
         apply (compatible_lockRes_sub_all _ H ) in juice_join0.
-        apply (mem_cohere_sub all_cohere0) in juice_join0.
+        assert (✓ all_juice) as Hv by (by destruct M as [[]]).
+        apply (mem_cohere_sub Hv all_cohere0) in juice_join0.
         assumption.
       Qed.
 
@@ -1833,132 +1662,9 @@ Qed.
         intros.
         inversion H as [all_juice M]; inversion M.
         eapply mem_cohere_sub.
+        - by destruct M as [[]].
         - eassumption.
         - apply compatible_threadRes_sub. assumption.
-      Qed.
-
-      (** *Lemmas about aging*)
-      Lemma cnt_age_iff {js i n} :
-          containsThread js i <->
-          containsThread (age_tp_to n js) i.
-      Proof.
-        destruct js; split; auto.
-      Qed.
-
-      Lemma gtc_age : forall js i n,
-          forall (cnt: containsThread js i)
-            (cnt': containsThread (age_tp_to n js) i),
-            getThreadC cnt = getThreadC cnt'.
-      Proof.
-        intros []. intros; simpl.
-        repeat f_equal; apply proof_irr.
-      Qed.
-
-      Lemma getThreadR_age: forall js i age,
-          forall (cnt: containsThread js i)
-            (cnt': containsThread (age_tp_to age js) i),
-            age_to age (getThreadR cnt) = getThreadR cnt'.
-      Proof.
-        intros. unfold getThreadR; destruct js; simpl.
-        unfold containsThread in cnt, cnt'.
-        simpl in cnt, cnt'.
-        unfold "oo";
-          do 3 f_equal. apply proof_irrelevance.
-      Qed.
-
-      Lemma LockRes_age: forall js age a,
-          isSome (lockRes (age_tp_to age js) a) = isSome (lockRes js a).
-      Proof.
-        destruct js.
-        intros; simpl. unfold OrdinalPool.lockRes; simpl.
-        destruct (AMap.find (elt:=option rmap) a
-                            (AMap.map (option_map (age_to age)) lset0)) eqn:AA;
-          destruct (AMap.find (elt:=option rmap) a lset0) eqn:BB;
-          try (reflexivity).
-        - apply AMap_find_map_inv in AA. destruct AA as [x [BB' rest]].
-          rewrite BB' in BB; inversion BB.
-        - apply AMap_find_map with (f:=(option_map (age_to age))) in BB.
-          rewrite BB in AA; inversion AA.
-      Qed.
-
-      Lemma LockRes_age_content1: forall js age a,
-          lockRes (age_tp_to age js) a = Some None ->
-          lockRes js a = Some None.
-        intros js age a. simpl; unfold OrdinalPool.lockRes; destruct js.
-        simpl.
-        intros AA.
-            apply AMap_find_map_inv in AA. destruct AA as [x [map rest]].
-            rewrite map. f_equal.
-            destruct x; inversion rest; try reflexivity.
-      Qed.
-
-      Lemma LockRes_age_content2: forall js age a rm,
-          lockRes (age_tp_to age js) a = Some (Some rm) ->
-          exists r, lockRes js a = Some (Some r) /\ rm = age_to age r.
-      Proof.
-        intros js age a rm. simpl; unfold OrdinalPool.lockRes; destruct js.
-        simpl.
-        intros AA.
-        apply AMap_find_map_inv in AA. destruct AA as [x [map rest]].
-        destruct x; inversion rest.
-        exists r; rewrite map; auto.
-      Qed.
-
-      Lemma access_cohere'_age m : hereditary age (access_cohere' m).
-      Proof.
-        intros x y E B.
-        intros addr.
-        destruct (age1_levelS _ _ E) as [n L].
-        eapply (age_age_to n) in E; auto.
-        rewrite <-E.
-        rewrite perm_of_age.
-        apply B.
-      Qed.
-
-      Lemma access_cohere'_unage m : hereditary unage (access_cohere' m).
-      Proof.
-        intros x y E B.
-        intros addr.
-        destruct (age1_levelS _ _ E) as [n L].
-        eapply (age_age_to n) in E; auto.
-        rewrite <-E in B.
-        specialize (B addr).
-        rewrite perm_of_age in B.
-        apply B.
-      Qed.
-
-      Lemma mem_cohere'_age m : hereditary age (mem_cohere' m).
-      Proof.
-        intros x y E.
-        intros [A B C]; constructor.
-        - eapply contents_cohere_age; eauto.
-       (* - eapply access_cohere'_age; eauto.*)
-        - eapply max_access_cohere_age; eauto.
-        - eapply alloc_cohere_age; eauto.
-      Qed.
-
-      Lemma mem_cohere'_unage m : hereditary unage (mem_cohere' m).
-      Proof.
-        intros x y E.
-        intros [A B C]; constructor.
-        - eapply contents_cohere_unage; eauto.
-        - eapply max_access_cohere_unage; eauto.
-        - eapply alloc_cohere_unage; eauto.
-      Qed.
-
-      Lemma mem_cohere_age_to n m phi :
-        mem_cohere' m phi ->
-        mem_cohere' m (age_to n phi).
-      Proof.
-        apply age_to_ind, mem_cohere'_age.
-      Qed.
-
-      Lemma mem_cohere_age_to_opp n m phi :
-        mem_cohere' m (age_to n phi) ->
-        mem_cohere' m phi.
-      Proof.
-        apply age_by_ind_opp.
-        intros x y A. apply mem_cohere'_unage, A.
       Qed.
 
     End JuicyMachineLemmas.
